plugin/src/automation/lift/liftrules.ml
@@ -188,6 +188,8 @@ let is_packed_constr c env sigma trm =
             sigma, None
        else
          sigma, None
+    | UnpackSigma ->
+       sigma, None
 
 (* Premises for LIFT-PACK *)
 let is_pack c env sigma trm =
@@ -207,11 +209,7 @@ let is_pack c env sigma trm =
          Util.on_snd Option.has_some (right_type trm)
        else
          sigma, false
-    | SwapConstruct _ ->
-       (* no packing *)
-       sigma, false
-    | CurryRecord ->
-       (* taken care of by constructor rule *)
+    | _ ->
        sigma, false
 
 (* Auxiliary function for premise for LIFT-PROJ *)
@@ -267,38 +265,41 @@ let is_proj c env trm =
 (* Premises for LIFT-ELIM *)
 let is_eliminator c env trm sigma =
   let l = get_lifting c in
-  match kind (first_fun trm) with
-  | Const (k, u) ->
-     let maybe_ind = inductive_of_elim env (k, u) in
-     if Option.has_some maybe_ind then
-       let ind = Option.get maybe_ind in
-       let is_elim = equal (mkInd (ind, 0)) (get_elim_type c) in
-       if is_elim then
-         let sigma, trm_eta = expand_eta env sigma trm in
-         let env_elim, trm_b = zoom_lambda_term env trm_eta in
-         let sigma, trm_elim = deconstruct_eliminator env_elim sigma trm_b in
-         if (not l.is_fwd) && l.orn.kind = CurryRecord then
-           let (final_args, post_args) = take_split 1 trm_elim.final_args in
-           let sigma, is_from = type_is_from c env_elim (List.hd final_args) sigma in
-           if Option.has_some is_from then
-             sigma, Some (env_elim, trm_eta, trm_elim, Option.get is_from)
+  if l.orn.kind = UnpackSigma then
+    sigma, None
+  else
+    match kind (first_fun trm) with
+    | Const (k, u) ->
+       let maybe_ind = inductive_of_elim env (k, u) in
+       if Option.has_some maybe_ind then
+         let ind = Option.get maybe_ind in
+         let is_elim = equal (mkInd (ind, 0)) (get_elim_type c) in
+         if is_elim then
+           let sigma, trm_eta = expand_eta env sigma trm in
+           let env_elim, trm_b = zoom_lambda_term env trm_eta in
+           let sigma, trm_elim = deconstruct_eliminator env_elim sigma trm_b in
+           if (not l.is_fwd) && l.orn.kind = CurryRecord then
+             let (final_args, post_args) = take_split 1 trm_elim.final_args in
+             let sigma, is_from = type_is_from c env_elim (List.hd final_args) sigma in
+             if Option.has_some is_from then
+               sigma, Some (env_elim, trm_eta, trm_elim, Option.get is_from)
+             else
+               sigma, None
            else
-             sigma, None
+             if l.orn.kind = CurryRecord then
+               let typ_f = first_fun (zoom_term zoom_lambda_term env_elim (snd (get_types c))) in
+               let sigma, to_typ_prod = specialize_delta_f env_elim typ_f trm_elim.pms sigma in
+               let to_elim = dest_prod to_typ_prod in
+               let pms = [to_elim.Produtils.typ1; to_elim.Produtils.typ2] in
+               sigma, Some (env_elim, trm_eta, trm_elim, pms)
+             else
+               sigma, Some (env_elim, trm_eta, trm_elim, trm_elim.pms)
          else
-           if l.orn.kind = CurryRecord then
-             let typ_f = first_fun (zoom_term zoom_lambda_term env_elim (snd (get_types c))) in
-             let sigma, to_typ_prod = specialize_delta_f env_elim typ_f trm_elim.pms sigma in
-             let to_elim = dest_prod to_typ_prod in
-             let pms = [to_elim.Produtils.typ1; to_elim.Produtils.typ2] in
-             sigma, Some (env_elim, trm_eta, trm_elim, pms)
-           else
-             sigma, Some (env_elim, trm_eta, trm_elim, trm_elim.pms)
+           sigma, None
        else
          sigma, None
-     else
+    | _ ->
        sigma, None
-  | _ ->
-     sigma, None
 
 (*
  * Given a term, determine the appropriate lift rule to run
